Model maps on top of only map values
Maps are basically only special in that they are sums (and nothing else
in the language is) and since they're recursive they need dedicated
typing rules.

src/go_lang/lang.v
@@ -95,9 +95,10 @@ Inductive bin_op : Set :=
   | AndOp | OrOp | XorOp (* Bitwise *)
   | ShiftLOp | ShiftROp (* Shifts *)
   | LeOp | LtOp | EqOp (* Relations *)
-  | OffsetOp. (* Pointer offset *)
+  | OffsetOp (* Pointer offset *)
+.
 
-Inductive arity : Set := args0 | args1 | args2 | args3.
+Inductive arity : Set := args0 | args1 | args2.
 
 Inductive prim_op : arity -> Set :=
   (* a stuck expression, to represent undefined behavior *)
@@ -106,8 +107,6 @@ Inductive prim_op : arity -> Set :=
   | AllocStructOp : prim_op args1 (* struct val *)
   | StoreOp : prim_op args2 (* pointer, value *)
   | LoadOp : prim_op args1
-  | MapGetOp : prim_op args2 (* map loc, key *)
-  | MapInsertOp : prim_op args3 (* map loc, key *)
   | EncodeInt64Op : prim_op args2 (* int, loc to store to *)
   | DecodeInt64Op : prim_op args1 (* loc to load from *)
   | EncodeInt32Op : prim_op args2 (* int, loc to store to *)
@@ -139,7 +138,7 @@ Inductive expr :=
   | Primitive0 (op: prim_op args0)
   | Primitive1 (op: prim_op args1) (e : expr)
   | Primitive2 (op: prim_op args2) (e1 e2 : expr)
-  | Primitive3 (op: prim_op args3) (e0 e1 e2 : expr)
+  (* | Primitive3 (op: prim_op args3) (e0 e1 e2 : expr) *)
   | CmpXchg (e0 : expr) (e1 : expr) (e2 : expr) (* Compare-exchange *)
   (* External FFI *)
   | ExternalOp (op: external) (e: expr)
@@ -162,8 +161,6 @@ Notation AllocN := (Primitive2 AllocNOp).
 Notation AllocStruct := (Primitive1 AllocStructOp).
 Notation Store := (Primitive2 StoreOp).
 Notation Load := (Primitive1 LoadOp).
-Notation MapGet := (Primitive2 MapGetOp).
-Notation MapInsert := (Primitive3 MapInsertOp).
 Notation EncodeInt64 := (Primitive2 EncodeInt64Op).
 Notation DecodeInt64 := (Primitive1 DecodeInt64Op).
 Notation EncodeInt32 := (Primitive2 EncodeInt32Op).
@@ -326,8 +323,8 @@ Proof using ext.
         cast_if_and (decide (op = op')) (decide (e = e'))
       | Primitive2 op e1 e2, Primitive2 op' e1' e2' =>
         cast_if_and3 (decide (op = op')) (decide (e1 = e1')) (decide (e2 = e2'))
-      | Primitive3 op e0 e1 e2, Primitive3 op' e0' e1' e2' =>
-        cast_if_and4 (decide (op = op')) (decide (e0 = e0')) (decide (e1 = e1')) (decide (e2 = e2'))
+      (* | Primitive3 op e0 e1 e2, Primitive3 op' e0' e1' e2' =>
+        cast_if_and4 (decide (op = op')) (decide (e0 = e0')) (decide (e1 = e1')) (decide (e2 = e2')) *)
       | UnOp o e, UnOp o' e' => cast_if_and (decide (o = o')) (decide (e = e'))
       | BinOp o e1 e2, BinOp o' e1' e2' =>
         cast_if_and3 (decide (o = o')) (decide (e1 = e1')) (decide (e2 = e2'))
@@ -450,8 +447,6 @@ Proof.
                                 | AllocStructOp => inr 7
                                 | StoreOp => inr 1
                                 | LoadOp => inr 2
-                                | MapGetOp => inr 3
-                                | MapInsertOp => inr 4
                                 | EncodeInt64Op => inr 5
                                 | DecodeInt64Op => inr 6
                                 | EncodeInt32Op => inr 8
@@ -463,8 +458,6 @@ Proof.
                                | inr 7 => a_prim_op AllocStructOp
                                | inr 1 => a_prim_op StoreOp
                                | inr 2 => a_prim_op LoadOp
-                               | inr 3 => a_prim_op MapGetOp
-                               | inr 4 => a_prim_op MapInsertOp
                                | inr 5 => a_prim_op EncodeInt64Op
                                | inr 6 => a_prim_op DecodeInt64Op
                                | inr 8 => a_prim_op EncodeInt32Op
@@ -537,7 +530,7 @@ Proof using ext.
      | Primitive0 op => GenNode 21 [GenLeaf $ primOpVal $ a_prim_op op]
      | Primitive1 op e => GenNode 22 [GenLeaf $ primOpVal $ a_prim_op op; go e]
      | Primitive2 op e1 e2 => GenNode 23 [GenLeaf $ primOpVal $ a_prim_op op; go e1; go e2]
-     | Primitive3 op e0 e1 e2 => GenNode 24 [GenLeaf $ primOpVal $ a_prim_op op; go e0; go e1; go e2]
+     (* | Primitive3 op e0 e1 e2 => GenNode 24 [GenLeaf $ primOpVal $ a_prim_op op; go e0; go e1; go e2] *)
      | UnOp op e => GenNode 3 [GenLeaf $ un_opVal op; go e]
      | BinOp op e1 e2 => GenNode 4 [GenLeaf $ bin_opVal op; go e1; go e2]
      | If e0 e1 e2 => GenNode 5 [go e0; go e1; go e2]
@@ -573,7 +566,7 @@ Proof using ext.
      | GenNode 21 [GenLeaf (primOpVal op)] => Primitive0 (`to_prim_op args0 op)
      | GenNode 22 [GenLeaf (primOpVal op); e] => Primitive1 (`to_prim_op args1 op) (go e)
      | GenNode 23 [GenLeaf (primOpVal op); e1; e2] => Primitive2 (`to_prim_op args2 op) (go e1) (go e2)
-     | GenNode 24 [GenLeaf (primOpVal op); e0; e1; e2] => Primitive3 (`to_prim_op args3 op) (go e0) (go e1) (go e2)
+     (* | GenNode 24 [GenLeaf (primOpVal op); e0; e1; e2] => Primitive3 (`to_prim_op args3 op) (go e0) (go e1) (go e2) *)
      | GenNode 3 [GenLeaf (un_opVal op); e] => UnOp op (go e)
      | GenNode 4 [GenLeaf (bin_opVal op); e1; e2] => BinOp op (go e1) (go e2)
      | GenNode 5 [e0; e1; e2] => If (go e0) (go e1) (go e2)
@@ -602,7 +595,7 @@ Proof using ext.
    for go).
  refine (inj_countable' enc dec _).
  refine (fix go (e : expr) {struct e} := _ with gov (v : val) {struct v} := _ for go).
-  - destruct e as [v| | | | | | | | | | | | | | | | | | | | |]; simpl; f_equal;
+  - destruct e as [v| | | | | | | | | | | | | | | | | | | |]; simpl; f_equal;
       rewrite ?to_prim_op_correct;
       [exact (gov v)|done..].
  - destruct v; by f_equal.
@@ -638,9 +631,9 @@ Inductive ectx_item :=
   | Primitive1Ctx  (op: prim_op args1)
   | Primitive2LCtx (op: prim_op args2) (v2 : val)
   | Primitive2RCtx (op: prim_op args2) (e1 : expr)
-  | Primitive3LCtx (op: prim_op args3) (e1 : expr) (e2 : expr)
+  (* | Primitive3LCtx (op: prim_op args3) (e1 : expr) (e2 : expr)
   | Primitive3MCtx (op: prim_op args3) (v0 : val) (e2 : expr)
-  | Primitive3RCtx (op: prim_op args3) (v0 : val) (v1 : val)
+  | Primitive3RCtx (op: prim_op args3) (v0 : val) (v1 : val) *)
   | ExternalOpCtx (op : external)
   | CmpXchgLCtx (e1 : expr) (e2 : expr)
   | CmpXchgMCtx (v1 : val) (e2 : expr)
@@ -674,9 +667,9 @@ Fixpoint fill_item (Ki : ectx_item) (e : expr) : expr :=
   | Primitive1Ctx op => Primitive1 op e
   | Primitive2LCtx op v2 => Primitive2 op e (Val v2)
   | Primitive2RCtx op e1 => Primitive2 op e1 e
-  | Primitive3LCtx op e1 e2 => Primitive3 op e e1 e2
+  (* | Primitive3LCtx op e1 e2 => Primitive3 op e e1 e2
   | Primitive3MCtx op v0 e1 => Primitive3 op (Val v0) e e1
-  | Primitive3RCtx op v0 v1 => Primitive3 op (Val v0) (Val v1) e
+  | Primitive3RCtx op v0 v1 => Primitive3 op (Val v0) (Val v1) e *)
   | ExternalOpCtx op => ExternalOp op e
   | CmpXchgLCtx e1 e2 => CmpXchg e e1 e2
   | CmpXchgMCtx v0 e2 => CmpXchg (Val v0) e e2
@@ -707,7 +700,7 @@ Fixpoint subst (x : string) (v : val) (e : expr)  : expr :=
   | Primitive0 op => Primitive0 op
   | Primitive1 op e => Primitive1 op (subst x v e)
   | Primitive2 op e1 e2 => Primitive2 op (subst x v e1) (subst x v e2)
-  | Primitive3 op e1 e2 e3 => Primitive3 op (subst x v e1) (subst x v e2) (subst x v e3)
+  (* | Primitive3 op e1 e2 e3 => Primitive3 op (subst x v e1) (subst x v e2) (subst x v e3) *)
   | ExternalOp op e => ExternalOp op (subst x v e)
   | CmpXchg e0 e1 e2 => CmpXchg (subst x v e0) (subst x v e1) (subst x v e2)
   | NewProph => NewProph
@@ -848,54 +841,6 @@ Proof.
   rewrite right_id insert_union_singleton_l. done.
 Qed.
 
-Notation MapConsV k v m := (InjRV (PairV (PairV (LitV (LitInt k)) v) m)).
-Notation MapNilV def := (InjLV def).
-
-Fixpoint map_val (v: val) : option (gmap u64 val * val) :=
-  match v with
-  | MapConsV k v m =>
-    match map_val m with
-    | Some (m, def) => Some (<[ k := v ]> m, def)
-    | None => None
-    end
-  | MapNilV def => Some (∅, def)
-  | _ => None
-  end.
-
-Definition val_of_map (m_def: gmap u64 val * val) : val :=
-  let (m, def) := m_def in
-  fold_right (λ '(k, v) mv, MapConsV k v mv)
-             (MapNilV def)
-             (map_to_list m).
-
-Theorem map_val_id : forall v m_def,
-    map_val v = Some m_def ->
-    val_of_map m_def = v.
-Proof.
-  induction v; intros [m def]; try solve [ inversion 1 ]; simpl; intros H.
-  - inversion H; subst; clear H.
-    rewrite map_to_list_empty; simpl; auto.
-  - destruct v; try congruence.
-    destruct v1; try congruence.
-    destruct v1_1; try congruence.
-    destruct l; try congruence.
-    destruct_with_eqn (map_val v2); try congruence.
-    specialize (IHv p).
-    destruct p as [m' def'].
-    inversion H; subst; clear H.
-    (* oops, the normal val induction principle is too weak to prove this *)
-Abort.
-
-Definition map_get (m_def: gmap u64 val * val) (k: u64) : (val*bool) :=
-  let (m, def) := m_def in
-  let r := default def (m !! k) in
-  let ok := bool_decide (is_Some (m !! k)) in
-  (r, ok).
-
-Definition map_insert (m_def: gmap u64 val * val) (k: u64) (v: val) : gmap u64 val * val :=
-  let (m, def) := m_def in
-  (<[ k := v ]> m, def).
-
 Definition byte_vals : list byte -> list val :=
    fmap (λ b, LitV (LitByte b)).
 
@@ -957,21 +902,6 @@ Inductive head_step : expr → state → list observation → expr → state →
      head_step (Store (Val $ LitV $ LitLoc l) (Val v)) σ
                []
                (Val $ LitV LitUnit) (state_upd_heap <[l:=v]> σ)
-               []
-  | MapGetS l k vs m_def r ok σ :
-     σ.(heap) !! l = Some vs ->
-     map_val vs = Some m_def ->
-     (r, ok) = map_get m_def k ->
-     head_step (MapGet (Val $ LitV $ LitLoc l) (Val $ LitV $ LitInt $ k)) σ
-               []
-               (Val $ PairV r (LitV $ LitBool ok)) σ
-               []
-  | MapInsertS l k vs v m_def σ :
-     σ.(heap) !! l = Some vs ->
-     map_val vs = Some m_def ->
-     head_step (MapInsert (Val $ LitV $ LitLoc l) (Val $ LitV $ LitInt $ k) (Val $ v)) σ
-               []
-               (Val $ LitV LitUnit) (state_upd_heap <[l := MapConsV k v vs ]> σ)
                []
   | ExternalS op v σ v' σ' :
      ext_step op v σ v' σ' ->
@@ -1134,8 +1064,6 @@ Notation AllocN := (Primitive2 AllocNOp).
 Notation AllocStruct := (Primitive1 AllocStructOp).
 Notation Store := (Primitive2 StoreOp).
 Notation Load := (Primitive1 LoadOp).
-Notation MapGet := (Primitive2 MapGetOp).
-Notation MapInsert := (Primitive3 MapInsertOp).
 Notation EncodeInt64 := (Primitive2 EncodeInt64Op).
 Notation DecodeInt64 := (Primitive1 DecodeInt64Op).
 Notation EncodeInt32 := (Primitive2 EncodeInt32Op).
