src/go_lang/map.v
@@ -1,0 +1,74 @@
+From stdpp Require Import fin_maps gmap.
+From Perennial.go_lang Require Import lang notation.
+
+Notation MapConsV k v m := (InjRV (PairV (PairV (LitV (LitInt k)) v) m)).
+Notation MapNilV def := (InjLV def).
+Notation AllocMap v := (Alloc (MapNilV v)) (only parsing).
+
+Section go_lang.
+  Context {ext:ext_op}.
+  Local Coercion Var' (s:string) : expr := Var s.
+
+Fixpoint map_val (v: val) : option (gmap u64 val * val) :=
+  match v with
+  | MapConsV k v m =>
+    match map_val m with
+    | Some (m, def) => Some (<[ k := v ]> m, def)
+    | None => None
+    end
+  | MapNilV def => Some (∅, def)
+  | _ => None
+  end.
+
+Definition val_of_map (m_def: gmap u64 val * val) : val :=
+  let (m, def) := m_def in
+  fold_right (λ '(k, v) mv, MapConsV k v mv)
+             (MapNilV def)
+             (map_to_list m).
+
+Theorem map_val_id : forall v m_def,
+    map_val v = Some m_def ->
+    val_of_map m_def = v.
+Proof.
+  induction v; intros [m def]; try solve [ inversion 1 ]; simpl; intros H.
+  - inversion H; subst; clear H.
+    rewrite map_to_list_empty; simpl; auto.
+  - destruct v; try congruence.
+    destruct v1; try congruence.
+    destruct v1_1; try congruence.
+    destruct l; try congruence.
+    destruct_with_eqn (map_val v2); try congruence.
+    specialize (IHv p).
+    destruct p as [m' def'].
+    inversion H; subst; clear H.
+    (* oops, the normal val induction principle is too weak to prove this *)
+Abort.
+
+Definition map_get (m_def: gmap u64 val * val) (k: u64) : (val*bool) :=
+  let (m, def) := m_def in
+  let r := default def (m !! k) in
+  let ok := bool_decide (is_Some (m !! k)) in
+  (r, ok).
+
+Definition map_insert (m_def: gmap u64 val * val) (k: u64) (v: val) : gmap u64 val * val :=
+  let (m, def) := m_def in
+  (<[ k := v ]> m, def).
+
+Definition MapGet: val :=
+  λ: "mref" "k",
+  let: "mapGet" := (rec: "mapGet" "m" :=
+                      match: "m" with
+                        InjL "def" => ("def", #false)
+                      | InjR "kvm" =>
+                        let: "kv" := Fst "kvm" in
+                        let: "m2" := Snd "kvm" in
+                        if: "k" = (Fst "kv") then (Snd "kv", #true)
+                        else "mapGet" "m2"
+                      end) in
+  "mapGet" !"mref".
+
+Definition MapInsert: val :=
+  λ: "mref" "k" "v",
+  "mref" <- InjR ("k", "v", !"mref").
+
+End go_lang.
