src/go_lang/prelude.v
@@ -1,5 +1,5 @@
 From Perennial.go_lang Require Export
-     lang notation slice struct typing.
+     lang notation slice map struct typing.
 
 (* We provide stubs here for primitive operations to make the Goose unit tests
    compile. *)
